Finished subst modulo admitted structural lemmas about contexts

TypedCircuits.v
@@ -16,12 +16,6 @@ Fixpoint interpret (w:WType) : Set :=
     | Tensor w1 w2 => (interpret w1) * (interpret w2)
   end.
 
-(*
-Inductive NCtx := 
-  End : WType -> NCtx
-| Cons : option WType -> NCtx -> NCtx.
-Inductive Ctx := Empty | NEmpty : NCtx -> Ctx.
-*)
 Definition Var := nat.
 Definition Ctx := list (option WType).
 
@@ -52,23 +46,6 @@ Inductive MergeCtx : Ctx -> Ctx -> Ctx -> Set :=
 | MergeCons : forall o1 o2 o g1 g2 g, 
               MergeOption o1 o2 o -> MergeCtx g1 g2 g -> MergeCtx (o1 :: g1) (o2 :: g2) (o :: g)
 .
-Fixpoint MergeOptionF (o1 : option WType) (o2 : option WType) 
-         : option (option WType) :=
-  match o1, o2 with
-  | None, _ => Some o2
-  | _, None => Some o1
-  | Some _, Some _ => None
-  end.
-Fixpoint MergeCtxF (Γ1 : Ctx) (Γ2 : Ctx) : option Ctx :=
-  match Γ1, Γ2 with
-  | [], _ => Some Γ2
-  | _, [] => Some Γ1
-  | (o1 :: Γ1'), (o2 :: Γ2') => 
-    match MergeOptionF o1 o2, MergeCtxF Γ1' Γ2' with
-    | Some o, Some Γ => Some (o :: Γ)
-    | _, _           => None
-    end
-  end.
 
 Inductive Pat : Ctx -> WType -> Set :=
 | var  : forall x w ctx, SingletonCtx x w ctx -> Pat ctx w
@@ -101,55 +78,39 @@ Definition unbox {ctx} {w1} {w2} (b : Box w1 w2) : Pat ctx w1 -> Circuit ctx w2 
   match b with
     box f => f ctx
   end.
-(*
-Program Fixpoint compose {ctx1} {w} (c : Circuit ctx1 w)
-                 : forall {ctx} {ctx1'} {w'}, 
-                  (forall ctx2 ctx2', MergeCtx ctx2 ctx ctx2'
-                                    -> Pat ctx2 w 
-                                    -> Circuit ctx2' w') 
-               -> MergeCtx ctx1 ctx ctx1' -> Circuit ctx1' w' :=
-  match c with
-    | output p1 => _
-    | gate ctx g p1 h pfM => _
-  end.
-*)
 
-Lemma mergeF : forall {Γ1 Γ2 Γ}, MergeCtxF Γ1 Γ2 = Some Γ -> MergeCtx Γ1 Γ2 Γ.
-Proof.
-  induction Γ1 as [ | o1 Γ1']; simpl; intros Γ2 Γ H; inversion H; subst; try constructor.
-  destruct Γ2 as [ | o2 Γ2']. inversion H; subst. constructor.
-  destruct o1; destruct o2; simpl in *; try (inversion H1; fail).
-  - remember (MergeCtxF Γ1' Γ2'). 
-    destruct o; simpl in *; try (inversion H1; fail).
-    inversion H; subst. constructor. constructor. apply IHΓ1'; auto.
-  - remember (MergeCtxF Γ1' Γ2'). 
-    destruct o; simpl in *; try (inversion H1; fail).
-    inversion H; subst. constructor. constructor. apply IHΓ1'; auto.
-  - remember (MergeCtxF Γ1' Γ2'). 
-    destruct o; simpl in *; try (inversion H1; fail).
-    inversion H; subst. constructor. constructor. apply IHΓ1'; auto.
-Qed.    
 Open Scope type_scope.
 
-Definition Disjoint Γ1 Γ2 := {Γ : Ctx & MergeCtxF Γ1 Γ2 = Some Γ}.
-Definition Subset Γ1 Γ := {Γ2 : Ctx & MergeCtxF Γ1 Γ2 = Some Γ}.
+Definition Disjoint Γ1 Γ2 := {Γ : Ctx & MergeCtx Γ1 Γ2 Γ}.
+Definition Subset Γ1 Γ := {Γ2 : Ctx & MergeCtx Γ1 Γ2 Γ}.
 
 Lemma mergeDisjoint : forall Γ1 Γ2 Γ3 Γ Γ',
       MergeCtx Γ1 Γ2 Γ -> MergeCtx Γ Γ3 Γ' -> Disjoint Γ1 Γ3 * Disjoint Γ2 Γ3.
 Admitted.
 
-Lemma disjointTrans : forall Γ1 Γ2 Γ Γ', MergeCtx Γ1 Γ2 Γ -> Disjoint Γ1 Γ' -> Disjoint Γ2 Γ' 
-                      -> Disjoint Γ Γ'.
+Lemma disjointTrans : forall Γ1 Γ2 Γ Γ', 
+      MergeCtx Γ1 Γ2 Γ -> Disjoint Γ1 Γ' -> Disjoint Γ2 Γ' -> Disjoint Γ Γ'.
 Admitted.
 
 Lemma mergeAssoc : forall Γ1 Γ2 Γ3 Γ Γ' Γ0,
       MergeCtx Γ1 Γ2 Γ -> MergeCtx Γ Γ3 Γ' 
-   -> MergeCtxF Γ2 Γ3 = Some Γ0
-   -> (MergeCtx Γ2 Γ3 Γ0) * (MergeCtx Γ1 Γ0 Γ').
+   -> MergeCtx Γ2 Γ3 Γ0
+   -> MergeCtx Γ1 Γ0 Γ'.
 Admitted.
 
 Lemma mergeSymm : forall {Γ1 Γ2 Γ}, MergeCtx Γ1 Γ2 Γ -> MergeCtx Γ2 Γ1 Γ.
 Admitted.
+
+Lemma mergeFunctional : forall {Γ1 Γ2 Γ Γ'}, 
+                 MergeCtx Γ1 Γ2 Γ -> MergeCtx Γ1 Γ2 Γ' -> Γ = Γ'.
+Admitted.
+
+
+Definition Merge3 Γ1 Γ2 Γ3 Γ := { Γ0 : Ctx & MergeCtx Γ1 Γ2 Γ0 * MergeCtx Γ0 Γ3 Γ}.
+Lemma merge3Assoc : forall Γ1 Γ2 Γ3 Γ,
+                    Merge3 Γ1 Γ2 Γ3 Γ -> Merge3 Γ1 Γ3 Γ2 Γ.
+Admitted.
+
 
 Fixpoint compose {Γ1} {W} (c : Circuit Γ1 W)
                  : forall {Γ} {Γ1'} {W'}, 
@@ -159,41 +120,32 @@ Fixpoint compose {Γ1} {W} (c : Circuit Γ1 W)
                -> MergeCtx Γ1 Γ Γ1' -> Circuit Γ1' W'.
   refine (match c with
             output p1 => fun Γ Γ1' W' f pfM => f _ _ pfM p1
-          | gate ctx g p1 h pfM => fun Γ Γ1' W' f pfM0 => _
+          | gate ctx g p1 h pfM' => fun Γ Γ1' W' f pfM => _
           end). 
-  clear W c Γ1.
-  rename w into W1, w0 into W2, w1 into W.
+  clear W c Γ1;
+  rename w into W1, w0 into W2, w1 into W;
   rename c0 into Γ01, c1 into Γ1, ctx into Γ0.
-  destruct (mergeDisjoint Γ01 Γ0 Γ Γ1 Γ1') as [[Γ01' pfM1] [Γ0' pfM2]]; auto.
-  destruct (mergeAssoc Γ01 Γ0 Γ Γ1 Γ1' Γ0') as [pfM3 pfM4]; auto.
-  refine (gate _ g p1 (fun Γ02 Γ02' pfM' q => _) pfM4);
-    destruct (mergeDisjoint Γ0 Γ Γ02 Γ0' Γ02') as [[Γ002 pfM6] [Γ02'' pfM5]];
-      try (auto; apply mergeSymm; auto).
-  refine (compose _ _ (h Γ02 Γ002 _ q) _ _ _ f _).
-  - apply mergeSymm. apply mergeF. apply pfM6.
-  - (* Γ002 = Γ0 ⋓ Γ02 *)
+  rename pfM' into Merge_Γ01_Γ0_Γ1, pfM into Merge_Γ1_Γ_Γ1'.
+  edestruct (mergeDisjoint Γ01 Γ0 Γ) as [Disj_Γ01_Γ Disj_Γ0_Γ]; eauto.
+  destruct Disj_Γ0_Γ as [Γ0' Merge_Γ0_Γ_Γ0'].
+  assert (Merge_Γ01_Γ0'_Γ1' : MergeCtx Γ01 Γ0' Γ1').
+    eapply mergeAssoc; eauto.
+  refine (gate _ g p1 (fun Γ02 Γ02' Merge_Γ02_Γ0'_Γ02' q => _) Merge_Γ01_Γ0'_Γ1').
+    edestruct (mergeDisjoint Γ0 Γ Γ02) as [[Γ002 Merge_Γ_Γ02_Γ002]
+                                           [Γ02'' Merge_Γ0_Γ002_Γ02'']]; eauto;
+      try (eapply mergeSymm; eauto; fail).
+  refine (compose _ _ (h Γ02 Γ002 _ q) _ _ _ f _);
+    try (apply mergeSymm; auto; fail).
+    (* Γ002 = Γ0 ⋓ Γ02 *)
     (* Γ02' = Γ02 ⋓ Γ0' = Γ02 ⋓ (Γ0 ⋓ Γ) *)
     (* So want to show that (Γ0 ⋓ Γ02) ⋓ Γ = Γ02 ⋓ (Γ0 ⋓ Γ) *)
-    (* First show that (Γ02 ⋓ Γ0) ⋓ Γ = Γ02 ⋓ (Γ0 ⋓ Γ) *)
-    (* Before that, show that Γ002 _|_ Γ *)
-    (* To do that, show that Γ0 _|_ Γ*) 
-    assert (pfDisjoint1 : Disjoint Γ0 Γ).
-      exists Γ0'; auto.
-    assert (pfDisjoint2 : Disjoint Γ02 Γ).
-      admit.
-    assert (pfDisjoint3 : Disjoint Γ002 Γ).
-      apply disjointTrans with (Γ1 := Γ0) (Γ2 := Γ02); auto. apply mergeF; auto.
-    destruct pfDisjoint1 as [ Γ0001 pfDisjoint1].
-    destruct pfDisjoint3 as [ Γ0002 pfDisjoint3]. 
-    (* as a result of mergeAssoc, we want Γ002 ⋓ Γ = Γ02' *)
+    assert (Merge3_Γ0_Γ_Γ02 : Merge3 Γ0 Γ Γ02 Γ02'). eexists.
+      constructor; eauto; try (apply mergeSymm; auto; fail).
+    apply merge3Assoc in Merge3_Γ0_Γ_Γ02.
+    destruct Merge3_Γ0_Γ_Γ02 as [Γ002' [Merge_Γ0_Γ02_Γ002' Merge_Γ002'_Γ_Γ02']].
+    assert (Γ002' = Γ002).
+      eapply mergeFunctional; eauto.
+    subst. auto.
+Qed.
 
-    edestruct (mergeAssoc Γ02 Γ0 Γ).
-    * eapply mergeSymm. eapply mergeF. eauto. 
-    * eapply mergeF. exact pfDisjoint3.
-    * exact pfDisjoint1.
-    * 
-    
-
-
-Admitted.
 
